# mist-team/mist

 @@ -0,0 +1,323 @@ \documentclass{article} \usepackage{epsfig} \pagestyle{empty} \begin{document} $\mbox{\boldmath p} = \mbox{\boldmath q} \rightarrow p_r = q_r \; \wedge \; p_g = q_g \; \wedge \; p_b = q_b$ \pagebreak $\mbox{\boldmath p} \neq \mbox{\boldmath q} \rightarrow \overline{ p_r = q_r \; \wedge \; p_g = q_g \; \wedge \; p_b = q_b }$ \pagebreak $\mbox{\boldmath p} \ge \mbox{\boldmath q} \rightarrow \overline{ p_r \ge q_r \; \wedge \; p_g \ge q_g \; \wedge \; p_b \ge q_b }$ \pagebreak $\mbox{\boldmath p} \le \mbox{\boldmath q} \rightarrow p_r \le q_r \; \wedge \; p_g \le q_g \; \wedge \; p_b \le q_b$ \pagebreak $\mbox{\boldmath p} \le \mbox{\boldmath q} \rightarrow \overline{ p_r \le q_r \; \wedge \; p_g \le q_g \; \wedge \; p_b \le q_b }$ \pagebreak $\mbox{\boldmath p} \ge \mbox{\boldmath q} \rightarrow p_r \ge q_r \; \wedge \; p_g \ge q_g \; \wedge \; p_b \ge q_b$ \pagebreak $a = b$ \pagebreak $a \neq b$ \pagebreak $a \subset b$ \pagebreak $a \subseteq b$ \pagebreak $a \supset b$ \pagebreak $a \supseteq b$ \pagebreak $a = a \bigcup b$ \pagebreak $a = a - \left( a \bigcap b \right)$ \pagebreak $a = a \bigcap b$ \pagebreak $\mbox{\boldmath p} = \mbox{\boldmath q} \rightarrow p_l = q_l \; \wedge \; p_r = q_r$ \pagebreak $\mbox{\boldmath p} \neq \mbox{\boldmath q} \rightarrow \overline{ p_l = q_l \; \wedge \; p_r = q_r }$ \pagebreak $\mbox{\boldmath p} \ge \mbox{\boldmath q} \rightarrow \overline{ p_l \ge q_l \; \wedge \; p_r \ge q_r }$ \pagebreak $\mbox{\boldmath p} \le \mbox{\boldmath q} \rightarrow p_l \le q_l \; \wedge \; p_r \le q_r$ \pagebreak $\mbox{\boldmath p} \le \mbox{\boldmath q} \rightarrow \overline{ p_l \le q_l \; \wedge \; p_r \le q_r }$ \pagebreak $\mbox{\boldmath p} \ge \mbox{\boldmath q} \rightarrow p_l \ge q_l \; \wedge \; p_r \ge q_r$ \pagebreak $l^2$ \pagebreak $a_x$ \pagebreak $l a_x$ \pagebreak $\left( \begin{array}{ccc} \sigma_1 & 0 & 0 \\ 0 & \sigma_2 & 0 \\ 0 & 0 & \sigma_3 \end{array} \right)$ \pagebreak $\sigma_1 \ge \sigma_2 \ge \sigma_3$ \pagebreak ${\bf A} = {\bf A} + {\bf B}$ \pagebreak ${\bf A} = {\bf A} - {\bf B}$ \pagebreak ${\bf A} = {\bf A} * {\bf B}$ \pagebreak ${\bf A} = {\bf A} + val * {\bf I}$ \pagebreak ${\bf A} = {\bf A} - val * {\bf I}$ \pagebreak ${\bf A} = {\bf A} * val$ \pagebreak ${\bf A} = {\bf A} / val$ \pagebreak $a \ge b \ge c$ \pagebreak $c \ge b \ge a$ \pagebreak $f(a)$ \pagebreak $f(b)$ \pagebreak $f(c)$ \pagebreak $\displaystyle-\min_{i} \left\{ -H_{ii} \right\}$ \pagebreak $\displaystyle\max_{i} \left\{ -H_{ii} + \sum_{i \ne j}{\|H_{ij}\|} \right\}$ \pagebreak ${\bf C} = \alpha \times {\bf A} \times {\bf B} + \beta \times {\bf C}$ \pagebreak ${\bf A}$ \pagebreak ${\bf B}$ \pagebreak ${\bf C}$ \pagebreak ${\bf C} = {\bf A} \times {\bf B}$ \pagebreak $tr\left( {\bf A} \right) = \sum^{n}_{i=1}{ a_{ii} }$ \pagebreak $tr\left( {\bf A} \right)$ \pagebreak $\left| {\bf A} \right| = \left| \begin{array}{ccccc} a_{11} & \cdots & a_{1j} & \cdots & a_{1n} \\ a_{21} & \cdots & a_{2j} & \cdots & a_{2n} \\ \vdots & \cdots & \vdots & \cdots & \vdots \\ a_{n1} & \cdots & a_{nj} & \cdots & a_{nn} \end{array} \right| = \sum^{n}_{j=1}{ \left( -1 \right)^{j+1} a_{1j} \left| \begin{array}{cccccc} a_{21} & \cdots & a_{2,j-1} & a_{2,j+1} & \cdots & a_{2n} \\ \vdots & \cdots & \vdots & \vdots & \cdots & \vdots \\ a_{n1} & \cdots & a_{n,j-1} & a_{n,j+1} & \cdots & a_{nn} \end{array} \right| }$ \pagebreak $\left| {\bf A} \right|$ \pagebreak ${\bf A}\mbox{\boldmath x} = \mbox{\boldmath b}$ \pagebreak $\mbox{\boldmath b}$ \pagebreak $\mbox{\boldmath x}$ \pagebreak ${\bf A} = {\bf P} \; \times \; {\bf L} \; \times \; {\bf U}$ \pagebreak $\mbox{\bf A}$ \pagebreak $\mbox{\bf L}$ \pagebreak $\mbox{\bf U}$ \pagebreak $\mbox{\bf P}$ \pagebreak ${\bf A} = {\bf Q} \; {\bf R}$ \pagebreak ${\bf A}^{-1}$ \pagebreak ${\bf A}^{-1}$ \pagebreak ${\bf A}\mbox{\boldmath x} = \lambda\mbox{\boldmath x}$ \pagebreak $\lambda$ \pagebreak ${\bf A} = {\bf U}{\bf \Sigma}{\bf V}^T$ \pagebreak ${\bf A}$ \pagebreak ${\bf U}$ \pagebreak ${\bf \Sigma}$ \pagebreak ${\bf V}^T$ \pagebreak $\mbox{\boldmath p} + \mbox{\boldmath q} = \left( p_w + q_w \;,\; p_x + q_x \;,\; p_y + q_y \;,\; p_z + q_z \right)^T$ \pagebreak $\mbox{\boldmath p} + a = \left( p_w + a \;,\; p_x \;,\; p_y \;,\; p_z \right)^T$ \pagebreak $\mbox{\boldmath p} - \mbox{\boldmath q} = \left( p_w - q_w \;,\; p_x - q_x \;,\; p_y - q_y \;,\; p_z - q_z \right)^T$ \pagebreak $\mbox{\boldmath p} - a = \left( p_w - a \;,\; p_x \;,\; p_y \;,\; p_z \right)^T$ \pagebreak $\mbox{\boldmath p} \times \mbox{\boldmath q} = \left( p_w \times q_w - p_x \times q_x - p_y \times q_y - p_z \times q_z \;,\; p_w \times q_x + p_x \times q_w + p_y \times q_z - p_z \times q_y \;,\; p_w \times q_y + p_y \times q_w + p_z \times q_x - p_x \times q_z \;,\; p_w \times q_z + p_z \times q_w + p_x \times q_y - p_y \times q_x \right)^T$ \pagebreak $\mbox{\boldmath p} \times a = \left( p_w \times a \;,\; p_x \times a \;,\; p_y \times a \;,\; p_z \times a \right)^T$ \pagebreak $\frac{ \mbox{\boldmath p} }{ \mbox{\boldmath q} } = \mbox{\boldmath p} \times \mbox{\boldmath q}^{-1}$ \pagebreak $\mbox{\boldmath p} \div a = \left( p_w \div a \;,\; p_x \div a \;,\; p_y \div a \;,\; p_z \div a \right)^T$ \pagebreak $\mbox{\boldmath p} == \mbox{\boldmath q} \rightarrow p_w == q_w \; \wedge \; p_x == q_x \; \wedge \; p_y == q_y \; \wedge \; p_z == q_z$ \pagebreak $\mbox{\boldmath p} \neq \mbox{\boldmath q} \rightarrow \overline{ p_w = q_w \; \wedge \; p_x = q_x \; \wedge \; p_y = q_y \; \wedge \; p_z = q_z }$ \pagebreak $\mbox{\boldmath p} < \mbox{\boldmath q} \rightarrow \overline{ p_w \ge q_w \; \wedge \; p_x \ge q_x \; \wedge \; p_y \ge q_y \; \wedge \; p_z \ge q_z }$ \pagebreak $\mbox{\boldmath p} \le \mbox{\boldmath q} \rightarrow p_w \le q_w \; \wedge \; p_x \le q_x \; \wedge \; p_y \le q_y \; \wedge \; p_z \le q_z$ \pagebreak $\mbox{\boldmath p} > \mbox{\boldmath q} \rightarrow \overline{ p_w \le q_w \; \wedge \; p_x \le q_x \; \wedge \; p_y \le q_y \; \wedge \; p_z \le q_z }$ \pagebreak $\mbox{\boldmath p} \ge \mbox{\boldmath q} \rightarrow p_w \ge q_w \; \wedge \; p_x \ge q_x \; \wedge \; p_y \ge q_y \; \wedge \; p_z \ge q_z$ \pagebreak $\overline{ \mbox{\boldmath p} } = \left( p_w \;,\; -p_x \;,\; -p_y \;,\; -p_z \right)^T$ \pagebreak $\mbox{\boldmath p}^{-1} = \frac{ \overline{ \mbox{\boldmath p} } }{ \left\| \mbox{\boldmath p} \right\|^2 }$ \pagebreak $\frac{ \mbox{\boldmath p} }{ \left\| \mbox{\boldmath p} \right\|^2 }$ \pagebreak $p_w \times q_w + p_x \times q_x + p_y \times q_y + p_z \times q_z$ \pagebreak $\left\| \mbox{\boldmath p} \right\| = \sqrt{ p_w^2 + p_x^2 + p_y^2 + p_z^2 }$ \pagebreak $\mbox{\boldmath p} = \mbox{\boldmath q} \rightarrow p_x = q_x \; \wedge \; p_y = q_y \; \wedge \; p_z = q_z$ \pagebreak $\mbox{\boldmath p} \neq \mbox{\boldmath q} \rightarrow \overline{ p_x = q_x \; \wedge \; p_y = q_y \; \wedge \; p_z = q_z}$ \pagebreak $\mbox{\boldmath p} \ge \mbox{\boldmath q} \rightarrow \overline{ p_x \ge q_x \; \wedge \; p_y \ge q_y \; \wedge \; p_z \ge q_z }$ \pagebreak $\mbox{\boldmath p} \le \mbox{\boldmath q} \rightarrow p_x \le q_x \; \wedge \; p_y \le q_y \; \wedge \; p_z \le q_z$ \pagebreak $\mbox{\boldmath p} \le \mbox{\boldmath q} \rightarrow \overline{ p_x \le q_x \; \wedge \; p_y \le q_y \; \wedge \; p_z \le q_z }$ \pagebreak $\mbox{\boldmath p} \ge \mbox{\boldmath q} \rightarrow p_x \ge q_x \; \wedge \; p_y \ge q_y \; \wedge \; p_z \ge q_z$ \pagebreak $\frac{\mbox{\boldmath v}}{\left\|{\mbox{\boldmath v}}\right\|}$ \pagebreak $\mbox{\boldmath p} \cdot \mbox{\boldmath q} = p_x \times q_x + p_y \times q_y + p_z \times q_z$ \pagebreak $\mbox{\boldmath p} \times \mbox{\boldmath q} = \left( p_y \times q_z - p_z \times q_y \;,\; p_z \times q_x - p_x \times q_z \;,\; p_x \times q_y - p_y \times q_x \right)^T$ \pagebreak $\left\|\mbox{\boldmath v}\right\| = \sqrt{v_x^2 + v_y^2 + v_z^2}$ \pagebreak $\mbox{\boldmath p} = \mbox{\boldmath q} \rightarrow p_x = q_x \; \wedge \; p_y = q_y$ \pagebreak $\mbox{\boldmath p} \neq \mbox{\boldmath q} \rightarrow \overline{ p_x = q_x \; \wedge \; p_y = q_y }$ \pagebreak $\mbox{\boldmath p} \ge \mbox{\boldmath q} \rightarrow \overline{ p_x \ge q_x \; \wedge \; p_y \ge q_y }$ \pagebreak $\mbox{\boldmath p} \ge \mbox{\boldmath q} \rightarrow p_x \le q_x \; \wedge \; p_y \le q_y$ \pagebreak $\mbox{\boldmath p} \ge \mbox{\boldmath q} \rightarrow \overline{ p_x \le q_x \; \wedge \; p_y \le q_y }$ \pagebreak $\mbox{\boldmath p} \ge \mbox{\boldmath q} \rightarrow p_x \ge q_x \; \wedge \; p_y \ge q_y$ \pagebreak $\frac{\mbox{\boldmath v}}{\left\|\mbox{\boldmath v}\right\|}$ \pagebreak $\mbox{\boldmath p} \cdot \mbox{\boldmath q} = p_x \times q_x + p_y \times q_y$ \pagebreak $\mbox{\boldmath p} \times \mbox{\boldmath q} = p_x \times q_y - p_y \times q_x$ \pagebreak $\left\|\mbox{\boldmath v}\right\| = \sqrt{v_x^2+v_y^2}$ \pagebreak \end{document}